Add loop proofs (#3)
These are complete proofs that the spec holds for the two loop
functions. The spec is also strengethened in order to be useful.

As yet no care has been taken to make sure the proofs are as smooth as
possible, just that they are proofs.

examples/e01/translation/Funs.lean
@@ -677,7 +677,7 @@ def U8.Insts.E01T : T Std.U8 := {
 }
 
 /-- [e01::__anodized_fn_ensures_f_loop::closure::{impl core::ops::function::FnMut<(&'_ u8,), bool> for e01::__anodized_fn_ensures_f_loop::closure::closure<'_0>}::call_mut]:
-    Source: 'examples/e01/src/lib.rs', lines 50:21-50:42 -/
+    Source: 'examples/e01/src/lib.rs', lines 52:21-52:42 -/
 def
   __anodized_fn_ensures_f_loop.closure.closure.Insts.CoreOpsFunctionFnMutTupleSharedU8Bool.call_mut
   (c : __anodized_fn_ensures_f_loop.closure.closure) (tupled_args : Std.U8) :
@@ -689,7 +689,7 @@ def
   ok (b, c)
 
 /-- [e01::__anodized_fn_ensures_f_loop::closure::{impl core::ops::function::FnOnce<(&'_ u8,), bool> for e01::__anodized_fn_ensures_f_loop::closure::closure<'_0>}::call_once]:
-    Source: 'examples/e01/src/lib.rs', lines 50:21-50:42 -/
+    Source: 'examples/e01/src/lib.rs', lines 52:21-52:42 -/
 def
   __anodized_fn_ensures_f_loop.closure.closure.Insts.CoreOpsFunctionFnOnceTupleSharedU8Bool.call_once
   (c : __anodized_fn_ensures_f_loop.closure.closure) (i : Std.U8) :
@@ -701,7 +701,7 @@ def
   ok b
 
 /-- Trait implementation: [e01::__anodized_fn_ensures_f_loop::closure::{impl core::ops::function::FnOnce<(&'_ u8,), bool> for e01::__anodized_fn_ensures_f_loop::closure::closure<'_0>}]
-    Source: 'examples/e01/src/lib.rs', lines 50:21-50:42 -/
+    Source: 'examples/e01/src/lib.rs', lines 52:21-52:42 -/
 @[reducible]
 def
   __anodized_fn_ensures_f_loop.closure.closure.Insts.CoreOpsFunctionFnOnceTupleSharedU8Bool
@@ -712,7 +712,7 @@ def
 }
 
 /-- Trait implementation: [e01::__anodized_fn_ensures_f_loop::closure::{impl core::ops::function::FnMut<(&'_ u8,), bool> for e01::__anodized_fn_ensures_f_loop::closure::closure<'_0>}]
-    Source: 'examples/e01/src/lib.rs', lines 50:21-50:42 -/
+    Source: 'examples/e01/src/lib.rs', lines 52:21-52:42 -/
 @[reducible]
 def
   __anodized_fn_ensures_f_loop.closure.closure.Insts.CoreOpsFunctionFnMutTupleSharedU8Bool
@@ -725,7 +725,7 @@ def
 }
 
 /-- [e01::__anodized_fn_ensures_f_loop::{impl core::ops::function::Fn<(&'_ u8,), bool> for e01::__anodized_fn_ensures_f_loop::closure<'_0>}::call]:
-    Source: 'examples/e01/src/lib.rs', lines 47:0-53:2 -/
+    Source: 'examples/e01/src/lib.rs', lines 50:0-55:2 -/
 def
   __anodized_fn_ensures_f_loop.closure.Insts.CoreOpsFunctionFnTupleSharedU8Bool.call
   (c : __anodized_fn_ensures_f_loop.closure) (tupled_args : Std.U8) :
@@ -739,7 +739,7 @@ def
   ok b
 
 /-- [e01::__anodized_fn_ensures_f_loop::{impl core::ops::function::FnMut<(&'_ u8,), bool> for e01::__anodized_fn_ensures_f_loop::closure<'_0>}::call_mut]:
-    Source: 'examples/e01/src/lib.rs', lines 47:0-53:2 -/
+    Source: 'examples/e01/src/lib.rs', lines 50:0-55:2 -/
 def
   __anodized_fn_ensures_f_loop.closure.Insts.CoreOpsFunctionFnMutTupleSharedU8Bool.call_mut
   (state : __anodized_fn_ensures_f_loop.closure) (args : Std.U8) :
@@ -751,7 +751,7 @@ def
   ok (b, state)
 
 /-- [e01::__anodized_fn_ensures_f_loop::{impl core::ops::function::FnOnce<(&'_ u8,), bool> for e01::__anodized_fn_ensures_f_loop::closure<'_0>}::call_once]:
-    Source: 'examples/e01/src/lib.rs', lines 47:0-53:2 -/
+    Source: 'examples/e01/src/lib.rs', lines 50:0-55:2 -/
 def
   __anodized_fn_ensures_f_loop.closure.Insts.CoreOpsFunctionFnOnceTupleSharedU8Bool.call_once
   (c : __anodized_fn_ensures_f_loop.closure) (i : Std.U8) : Result Bool := do
@@ -761,7 +761,7 @@ def
   ok b
 
 /-- Trait implementation: [e01::__anodized_fn_ensures_f_loop::{impl core::ops::function::FnOnce<(&'_ u8,), bool> for e01::__anodized_fn_ensures_f_loop::closure<'_0>}]
-    Source: 'examples/e01/src/lib.rs', lines 47:0-53:2 -/
+    Source: 'examples/e01/src/lib.rs', lines 50:0-55:2 -/
 @[reducible]
 def
   __anodized_fn_ensures_f_loop.closure.Insts.CoreOpsFunctionFnOnceTupleSharedU8Bool
@@ -772,7 +772,7 @@ def
 }
 
 /-- Trait implementation: [e01::__anodized_fn_ensures_f_loop::{impl core::ops::function::FnMut<(&'_ u8,), bool> for e01::__anodized_fn_ensures_f_loop::closure<'_0>}]
-    Source: 'examples/e01/src/lib.rs', lines 47:0-53:2 -/
+    Source: 'examples/e01/src/lib.rs', lines 50:0-55:2 -/
 @[reducible]
 def
   __anodized_fn_ensures_f_loop.closure.Insts.CoreOpsFunctionFnMutTupleSharedU8Bool
@@ -785,7 +785,7 @@ def
 }
 
 /-- Trait implementation: [e01::__anodized_fn_ensures_f_loop::{impl core::ops::function::Fn<(&'_ u8,), bool> for e01::__anodized_fn_ensures_f_loop::closure<'_0>}]
-    Source: 'examples/e01/src/lib.rs', lines 47:0-53:2 -/
+    Source: 'examples/e01/src/lib.rs', lines 50:0-55:2 -/
 @[reducible]
 def
   __anodized_fn_ensures_f_loop.closure.Insts.CoreOpsFunctionFnTupleSharedU8Bool
@@ -796,25 +796,101 @@ def
     __anodized_fn_ensures_f_loop.closure.Insts.CoreOpsFunctionFnTupleSharedU8Bool.call
 }
 
+/-- [e01::__anodized_fn_ensures_f_loop::{impl core::ops::function::Fn<(&'_ u8,), bool> for e01::__anodized_fn_ensures_f_loop::closure#1<'_0>}::call]:
+    Source: 'examples/e01/src/lib.rs', lines 50:0-55:2 -/
+def
+  __anodized_fn_ensures_f_loop.closure_1.Insts.CoreOpsFunctionFnTupleSharedU8Bool.call
+  (c : __anodized_fn_ensures_f_loop.closure_1) (tupled_args : Std.U8) :
+  Result Bool
+  := do
+  let b ← core.slice.Slice.contains core.cmp.PartialEqU8 c tupled_args
+  let i := Slice.len c
+  ok (b = (i > 0#usize))
+
+/-- [e01::__anodized_fn_ensures_f_loop::{impl core::ops::function::FnMut<(&'_ u8,), bool> for e01::__anodized_fn_ensures_f_loop::closure#1<'_0>}::call_mut]:
+    Source: 'examples/e01/src/lib.rs', lines 50:0-55:2 -/
+def
+  __anodized_fn_ensures_f_loop.closure_1.Insts.CoreOpsFunctionFnMutTupleSharedU8Bool.call_mut
+  (state : __anodized_fn_ensures_f_loop.closure_1) (args : Std.U8) :
+  Result (Bool × __anodized_fn_ensures_f_loop.closure_1)
+  := do
+  let b ←
+    __anodized_fn_ensures_f_loop.closure_1.Insts.CoreOpsFunctionFnTupleSharedU8Bool.call
+      state args
+  ok (b, state)
+
+/-- [e01::__anodized_fn_ensures_f_loop::{impl core::ops::function::FnOnce<(&'_ u8,), bool> for e01::__anodized_fn_ensures_f_loop::closure#1<'_0>}::call_once]:
+    Source: 'examples/e01/src/lib.rs', lines 50:0-55:2 -/
+def
+  __anodized_fn_ensures_f_loop.closure_1.Insts.CoreOpsFunctionFnOnceTupleSharedU8Bool.call_once
+  (c : __anodized_fn_ensures_f_loop.closure_1) (i : Std.U8) : Result Bool := do
+  let (b, _) ←
+    __anodized_fn_ensures_f_loop.closure_1.Insts.CoreOpsFunctionFnMutTupleSharedU8Bool.call_mut
+      c i
+  ok b
+
+/-- Trait implementation: [e01::__anodized_fn_ensures_f_loop::{impl core::ops::function::FnOnce<(&'_ u8,), bool> for e01::__anodized_fn_ensures_f_loop::closure#1<'_0>}]
+    Source: 'examples/e01/src/lib.rs', lines 50:0-55:2 -/
+@[reducible]
+def
+  __anodized_fn_ensures_f_loop.closure_1.Insts.CoreOpsFunctionFnOnceTupleSharedU8Bool
+  : core.ops.function.FnOnce __anodized_fn_ensures_f_loop.closure_1 Std.U8 Bool
+  := {
+  call_once :=
+    __anodized_fn_ensures_f_loop.closure_1.Insts.CoreOpsFunctionFnOnceTupleSharedU8Bool.call_once
+}
+
+/-- Trait implementation: [e01::__anodized_fn_ensures_f_loop::{impl core::ops::function::FnMut<(&'_ u8,), bool> for e01::__anodized_fn_ensures_f_loop::closure#1<'_0>}]
+    Source: 'examples/e01/src/lib.rs', lines 50:0-55:2 -/
+@[reducible]
+def
+  __anodized_fn_ensures_f_loop.closure_1.Insts.CoreOpsFunctionFnMutTupleSharedU8Bool
+  : core.ops.function.FnMut __anodized_fn_ensures_f_loop.closure_1 Std.U8 Bool
+  := {
+  FnOnceInst :=
+    __anodized_fn_ensures_f_loop.closure_1.Insts.CoreOpsFunctionFnOnceTupleSharedU8Bool
+  call_mut :=
+    __anodized_fn_ensures_f_loop.closure_1.Insts.CoreOpsFunctionFnMutTupleSharedU8Bool.call_mut
+}
+
+/-- Trait implementation: [e01::__anodized_fn_ensures_f_loop::{impl core::ops::function::Fn<(&'_ u8,), bool> for e01::__anodized_fn_ensures_f_loop::closure#1<'_0>}]
+    Source: 'examples/e01/src/lib.rs', lines 50:0-55:2 -/
+@[reducible]
+def
+  __anodized_fn_ensures_f_loop.closure_1.Insts.CoreOpsFunctionFnTupleSharedU8Bool
+  : core.ops.function.Fn __anodized_fn_ensures_f_loop.closure_1 Std.U8 Bool
+  := {
+  FnMutInst :=
+    __anodized_fn_ensures_f_loop.closure_1.Insts.CoreOpsFunctionFnMutTupleSharedU8Bool
+  call :=
+    __anodized_fn_ensures_f_loop.closure_1.Insts.CoreOpsFunctionFnTupleSharedU8Bool.call
+}
+
 /-- [e01::__anodized_fn_requires_f_loop]:
-    Source: 'examples/e01/src/lib.rs', lines 47:0-53:2 -/
+    Source: 'examples/e01/src/lib.rs', lines 50:0-55:2 -/
 def __anodized_fn_requires_f_loop (x : Slice Std.U8) : Result Bool := do
   ok true
 
 /-- [e01::__anodized_fn_ensures_f_loop]:
-    Source: 'examples/e01/src/lib.rs', lines 47:0-53:2 -/
+    Source: 'examples/e01/src/lib.rs', lines 50:0-55:2 -/
 def __anodized_fn_ensures_f_loop
   (x : Slice Std.U8) (__anodized_output : Std.U8) : Result Bool := do
-  __anodized_fn_ensures_f_loop.closure.Insts.CoreOpsFunctionFnTupleSharedU8Bool.call
-    x __anodized_output
+  let b ←
+    __anodized_fn_ensures_f_loop.closure.Insts.CoreOpsFunctionFnTupleSharedU8Bool.call
+      x __anodized_output
+  if b
+  then
+    __anodized_fn_ensures_f_loop.closure_1.Insts.CoreOpsFunctionFnTupleSharedU8Bool.call
+      x __anodized_output
+  else ok false
 
 /-- [e01::__anodized_fn_qualifiers_f_loop]
-    Source: 'examples/e01/src/lib.rs', lines 47:0-53:2 -/
+    Source: 'examples/e01/src/lib.rs', lines 50:0-55:2 -/
 @[global_simps, irreducible]
 def __anodized_fn_qualifiers_f_loop : Std.U32 := 0#u32
 
 /-- [e01::f_loop]: loop body 0:
-    Source: 'examples/e01/src/lib.rs', lines 59:4-63:5
+    Source: 'examples/e01/src/lib.rs', lines 61:4-65:5
     Visibility: public -/
 @[rust_loop_body]
 def f_loop_loop.body
@@ -832,7 +908,7 @@ def f_loop_loop.body
     else ok (cont (iter1, max))
 
 /-- [e01::f_loop]: loop 0:
-    Source: 'examples/e01/src/lib.rs', lines 59:4-63:5
+    Source: 'examples/e01/src/lib.rs', lines 61:4-65:5
     Visibility: public -/
 @[rust_loop]
 def f_loop_loop
@@ -844,14 +920,14 @@ def f_loop_loop
     (iter, max)
 
 /-- [e01::f_loop]:
-    Source: 'examples/e01/src/lib.rs', lines 54:0-65:1
+    Source: 'examples/e01/src/lib.rs', lines 56:0-67:1
     Visibility: public -/
 def f_loop (x : Slice Std.U8) : Result Std.U8 := do
   let i := Slice.len x
   f_loop_loop { start := 0#usize, «end» := i } x 0#u8
 
 /-- [e01::__anodized_fn_ensures_f_while::closure::{impl core::ops::function::FnMut<(&'_ u8,), bool> for e01::__anodized_fn_ensures_f_while::closure::closure<'_0>}::call_mut]:
-    Source: 'examples/e01/src/lib.rs', lines 72:21-72:42 -/
+    Source: 'examples/e01/src/lib.rs', lines 73:21-73:42 -/
 def
   __anodized_fn_ensures_f_while.closure.closure.Insts.CoreOpsFunctionFnMutTupleSharedU8Bool.call_mut
   (c : __anodized_fn_ensures_f_while.closure.closure) (tupled_args : Std.U8) :
@@ -863,7 +939,7 @@ def
   ok (b, c)
 
 /-- [e01::__anodized_fn_ensures_f_while::closure::{impl core::ops::function::FnOnce<(&'_ u8,), bool> for e01::__anodized_fn_ensures_f_while::closure::closure<'_0>}::call_once]:
-    Source: 'examples/e01/src/lib.rs', lines 72:21-72:42 -/
+    Source: 'examples/e01/src/lib.rs', lines 73:21-73:42 -/
 def
   __anodized_fn_ensures_f_while.closure.closure.Insts.CoreOpsFunctionFnOnceTupleSharedU8Bool.call_once
   (c : __anodized_fn_ensures_f_while.closure.closure) (i : Std.U8) :
@@ -875,7 +951,7 @@ def
   ok b
 
 /-- Trait implementation: [e01::__anodized_fn_ensures_f_while::closure::{impl core::ops::function::FnOnce<(&'_ u8,), bool> for e01::__anodized_fn_ensures_f_while::closure::closure<'_0>}]
-    Source: 'examples/e01/src/lib.rs', lines 72:21-72:42 -/
+    Source: 'examples/e01/src/lib.rs', lines 73:21-73:42 -/
 @[reducible]
 def
   __anodized_fn_ensures_f_while.closure.closure.Insts.CoreOpsFunctionFnOnceTupleSharedU8Bool
@@ -886,7 +962,7 @@ def
 }
 
 /-- Trait implementation: [e01::__anodized_fn_ensures_f_while::closure::{impl core::ops::function::FnMut<(&'_ u8,), bool> for e01::__anodized_fn_ensures_f_while::closure::closure<'_0>}]
-    Source: 'examples/e01/src/lib.rs', lines 72:21-72:42 -/
+    Source: 'examples/e01/src/lib.rs', lines 73:21-73:42 -/
 @[reducible]
 def
   __anodized_fn_ensures_f_while.closure.closure.Insts.CoreOpsFunctionFnMutTupleSharedU8Bool
@@ -899,7 +975,7 @@ def
 }
 
 /-- [e01::__anodized_fn_ensures_f_while::{impl core::ops::function::Fn<(&'_ u8,), bool> for e01::__anodized_fn_ensures_f_while::closure<'_0>}::call]:
-    Source: 'examples/e01/src/lib.rs', lines 69:0-75:2 -/
+    Source: 'examples/e01/src/lib.rs', lines 71:0-76:2 -/
 def
   __anodized_fn_ensures_f_while.closure.Insts.CoreOpsFunctionFnTupleSharedU8Bool.call
   (c : __anodized_fn_ensures_f_while.closure) (tupled_args : Std.U8) :
@@ -913,7 +989,7 @@ def
   ok b
 
 /-- [e01::__anodized_fn_ensures_f_while::{impl core::ops::function::FnMut<(&'_ u8,), bool> for e01::__anodized_fn_ensures_f_while::closure<'_0>}::call_mut]:
-    Source: 'examples/e01/src/lib.rs', lines 69:0-75:2 -/
+    Source: 'examples/e01/src/lib.rs', lines 71:0-76:2 -/
 def
   __anodized_fn_ensures_f_while.closure.Insts.CoreOpsFunctionFnMutTupleSharedU8Bool.call_mut
   (state : __anodized_fn_ensures_f_while.closure) (args : Std.U8) :
@@ -925,7 +1001,7 @@ def
   ok (b, state)
 
 /-- [e01::__anodized_fn_ensures_f_while::{impl core::ops::function::FnOnce<(&'_ u8,), bool> for e01::__anodized_fn_ensures_f_while::closure<'_0>}::call_once]:
-    Source: 'examples/e01/src/lib.rs', lines 69:0-75:2 -/
+    Source: 'examples/e01/src/lib.rs', lines 71:0-76:2 -/
 def
   __anodized_fn_ensures_f_while.closure.Insts.CoreOpsFunctionFnOnceTupleSharedU8Bool.call_once
   (c : __anodized_fn_ensures_f_while.closure) (i : Std.U8) : Result Bool := do
@@ -935,7 +1011,7 @@ def
   ok b
 
 /-- Trait implementation: [e01::__anodized_fn_ensures_f_while::{impl core::ops::function::FnOnce<(&'_ u8,), bool> for e01::__anodized_fn_ensures_f_while::closure<'_0>}]
-    Source: 'examples/e01/src/lib.rs', lines 69:0-75:2 -/
+    Source: 'examples/e01/src/lib.rs', lines 71:0-76:2 -/
 @[reducible]
 def
   __anodized_fn_ensures_f_while.closure.Insts.CoreOpsFunctionFnOnceTupleSharedU8Bool
@@ -946,7 +1022,7 @@ def
 }
 
 /-- Trait implementation: [e01::__anodized_fn_ensures_f_while::{impl core::ops::function::FnMut<(&'_ u8,), bool> for e01::__anodized_fn_ensures_f_while::closure<'_0>}]
-    Source: 'examples/e01/src/lib.rs', lines 69:0-75:2 -/
+    Source: 'examples/e01/src/lib.rs', lines 71:0-76:2 -/
 @[reducible]
 def
   __anodized_fn_ensures_f_while.closure.Insts.CoreOpsFunctionFnMutTupleSharedU8Bool
@@ -959,7 +1035,7 @@ def
 }
 
 /-- Trait implementation: [e01::__anodized_fn_ensures_f_while::{impl core::ops::function::Fn<(&'_ u8,), bool> for e01::__anodized_fn_ensures_f_while::closure<'_0>}]
-    Source: 'examples/e01/src/lib.rs', lines 69:0-75:2 -/
+    Source: 'examples/e01/src/lib.rs', lines 71:0-76:2 -/
 @[reducible]
 def
   __anodized_fn_ensures_f_while.closure.Insts.CoreOpsFunctionFnTupleSharedU8Bool
@@ -970,25 +1046,103 @@ def
     __anodized_fn_ensures_f_while.closure.Insts.CoreOpsFunctionFnTupleSharedU8Bool.call
 }
 
+/-- [e01::__anodized_fn_ensures_f_while::{impl core::ops::function::Fn<(&'_ u8,), bool> for e01::__anodized_fn_ensures_f_while::closure#1<'_0>}::call]:
+    Source: 'examples/e01/src/lib.rs', lines 71:0-76:2 -/
+def
+  __anodized_fn_ensures_f_while.closure_1.Insts.CoreOpsFunctionFnTupleSharedU8Bool.call
+  (c : __anodized_fn_ensures_f_while.closure_1) (tupled_args : Std.U8) :
+  Result Bool
+  := do
+  let b ← core.slice.Slice.contains core.cmp.PartialEqU8 c tupled_args
+  let i := Slice.len c
+  ok (b = (i > 0#usize))
+
+/-- [e01::__anodized_fn_ensures_f_while::{impl core::ops::function::FnMut<(&'_ u8,), bool> for e01::__anodized_fn_ensures_f_while::closure#1<'_0>}::call_mut]:
+    Source: 'examples/e01/src/lib.rs', lines 71:0-76:2 -/
+def
+  __anodized_fn_ensures_f_while.closure_1.Insts.CoreOpsFunctionFnMutTupleSharedU8Bool.call_mut
+  (state : __anodized_fn_ensures_f_while.closure_1) (args : Std.U8) :
+  Result (Bool × __anodized_fn_ensures_f_while.closure_1)
+  := do
+  let b ←
+    __anodized_fn_ensures_f_while.closure_1.Insts.CoreOpsFunctionFnTupleSharedU8Bool.call
+      state args
+  ok (b, state)
+
+/-- [e01::__anodized_fn_ensures_f_while::{impl core::ops::function::FnOnce<(&'_ u8,), bool> for e01::__anodized_fn_ensures_f_while::closure#1<'_0>}::call_once]:
+    Source: 'examples/e01/src/lib.rs', lines 71:0-76:2 -/
+def
+  __anodized_fn_ensures_f_while.closure_1.Insts.CoreOpsFunctionFnOnceTupleSharedU8Bool.call_once
+  (c : __anodized_fn_ensures_f_while.closure_1) (i : Std.U8) :
+  Result Bool
+  := do
+  let (b, _) ←
+    __anodized_fn_ensures_f_while.closure_1.Insts.CoreOpsFunctionFnMutTupleSharedU8Bool.call_mut
+      c i
+  ok b
+
+/-- Trait implementation: [e01::__anodized_fn_ensures_f_while::{impl core::ops::function::FnOnce<(&'_ u8,), bool> for e01::__anodized_fn_ensures_f_while::closure#1<'_0>}]
+    Source: 'examples/e01/src/lib.rs', lines 71:0-76:2 -/
+@[reducible]
+def
+  __anodized_fn_ensures_f_while.closure_1.Insts.CoreOpsFunctionFnOnceTupleSharedU8Bool
+  : core.ops.function.FnOnce __anodized_fn_ensures_f_while.closure_1 Std.U8
+  Bool := {
+  call_once :=
+    __anodized_fn_ensures_f_while.closure_1.Insts.CoreOpsFunctionFnOnceTupleSharedU8Bool.call_once
+}
+
+/-- Trait implementation: [e01::__anodized_fn_ensures_f_while::{impl core::ops::function::FnMut<(&'_ u8,), bool> for e01::__anodized_fn_ensures_f_while::closure#1<'_0>}]
+    Source: 'examples/e01/src/lib.rs', lines 71:0-76:2 -/
+@[reducible]
+def
+  __anodized_fn_ensures_f_while.closure_1.Insts.CoreOpsFunctionFnMutTupleSharedU8Bool
+  : core.ops.function.FnMut __anodized_fn_ensures_f_while.closure_1 Std.U8 Bool
+  := {
+  FnOnceInst :=
+    __anodized_fn_ensures_f_while.closure_1.Insts.CoreOpsFunctionFnOnceTupleSharedU8Bool
+  call_mut :=
+    __anodized_fn_ensures_f_while.closure_1.Insts.CoreOpsFunctionFnMutTupleSharedU8Bool.call_mut
+}
+
+/-- Trait implementation: [e01::__anodized_fn_ensures_f_while::{impl core::ops::function::Fn<(&'_ u8,), bool> for e01::__anodized_fn_ensures_f_while::closure#1<'_0>}]
+    Source: 'examples/e01/src/lib.rs', lines 71:0-76:2 -/
+@[reducible]
+def
+  __anodized_fn_ensures_f_while.closure_1.Insts.CoreOpsFunctionFnTupleSharedU8Bool
+  : core.ops.function.Fn __anodized_fn_ensures_f_while.closure_1 Std.U8 Bool
+  := {
+  FnMutInst :=
+    __anodized_fn_ensures_f_while.closure_1.Insts.CoreOpsFunctionFnMutTupleSharedU8Bool
+  call :=
+    __anodized_fn_ensures_f_while.closure_1.Insts.CoreOpsFunctionFnTupleSharedU8Bool.call
+}
+
 /-- [e01::__anodized_fn_requires_f_while]:
-    Source: 'examples/e01/src/lib.rs', lines 69:0-75:2 -/
+    Source: 'examples/e01/src/lib.rs', lines 71:0-76:2 -/
 def __anodized_fn_requires_f_while (x : Slice Std.U8) : Result Bool := do
   ok true
 
 /-- [e01::__anodized_fn_ensures_f_while]:
-    Source: 'examples/e01/src/lib.rs', lines 69:0-75:2 -/
+    Source: 'examples/e01/src/lib.rs', lines 71:0-76:2 -/
 def __anodized_fn_ensures_f_while
   (x : Slice Std.U8) (__anodized_output : Std.U8) : Result Bool := do
-  __anodized_fn_ensures_f_while.closure.Insts.CoreOpsFunctionFnTupleSharedU8Bool.call
-    x __anodized_output
+  let b ←
+    __anodized_fn_ensures_f_while.closure.Insts.CoreOpsFunctionFnTupleSharedU8Bool.call
+      x __anodized_output
+  if b
+  then
+    __anodized_fn_ensures_f_while.closure_1.Insts.CoreOpsFunctionFnTupleSharedU8Bool.call
+      x __anodized_output
+  else ok false
 
 /-- [e01::__anodized_fn_qualifiers_f_while]
-    Source: 'examples/e01/src/lib.rs', lines 69:0-75:2 -/
+    Source: 'examples/e01/src/lib.rs', lines 71:0-76:2 -/
 @[global_simps, irreducible]
 def __anodized_fn_qualifiers_f_while : Std.U32 := 0#u32
 
 /-- [e01::f_while]: loop body 0:
-    Source: 'examples/e01/src/lib.rs', lines 86:4-91:5
+    Source: 'examples/e01/src/lib.rs', lines 87:4-92:5
     Visibility: public -/
 @[rust_loop_body]
 def f_while_loop.body
@@ -1007,7 +1161,7 @@ def f_while_loop.body
   else ok (done max)
 
 /-- [e01::f_while]: loop 0:
-    Source: 'examples/e01/src/lib.rs', lines 86:4-91:5
+    Source: 'examples/e01/src/lib.rs', lines 87:4-92:5
     Visibility: public -/
 @[rust_loop]
 def f_while_loop
@@ -1017,20 +1171,20 @@ def f_while_loop
     (max, i)
 
 /-- [e01::f_while]:
-    Source: 'examples/e01/src/lib.rs', lines 76:0-93:1
+    Source: 'examples/e01/src/lib.rs', lines 77:0-94:1
     Visibility: public -/
 @[reducible]
 def f_while (x : Slice Std.U8) : Result Std.U8 := do
   f_while_loop x 0#u8 0#usize
 
 /-- [e01::{e01::S}::__anodized_data_maintains::{impl core::ops::function::Fn<(), bool> for e01::{e01::S}::__anodized_data_maintains::closure<'_0>}::call]:
-    Source: 'examples/e01/src/lib.rs', lines 97:0-99:2 -/
+    Source: 'examples/e01/src/lib.rs', lines 98:0-100:2 -/
 def S.__anodized_data_maintains.closure.Insts.CoreOpsFunctionFnTupleBool.call
   (c : S.__anodized_data_maintains.closure) (_ : Unit) : Result Bool := do
   ok (c.x > 0#u8)
 
 /-- [e01::{e01::S}::__anodized_data_maintains::{impl core::ops::function::FnMut<(), bool> for e01::{e01::S}::__anodized_data_maintains::closure<'_0>}::call_mut]:
-    Source: 'examples/e01/src/lib.rs', lines 97:0-99:2 -/
+    Source: 'examples/e01/src/lib.rs', lines 98:0-100:2 -/
 def
   S.__anodized_data_maintains.closure.Insts.CoreOpsFunctionFnMutTupleBool.call_mut
   (state : S.__anodized_data_maintains.closure) (_ : Unit) :
@@ -1042,7 +1196,7 @@ def
   ok (b, state)
 
 /-- [e01::{e01::S}::__anodized_data_maintains::{impl core::ops::function::FnOnce<(), bool> for e01::{e01::S}::__anodized_data_maintains::closure<'_0>}::call_once]:
-    Source: 'examples/e01/src/lib.rs', lines 97:0-99:2 -/
+    Source: 'examples/e01/src/lib.rs', lines 98:0-100:2 -/
 def
   S.__anodized_data_maintains.closure.Insts.CoreOpsFunctionFnOnceTupleBool.call_once
   (c : S.__anodized_data_maintains.closure) (_ : Unit) : Result Bool := do
@@ -1052,7 +1206,7 @@ def
   ok b
 
 /-- Trait implementation: [e01::{e01::S}::__anodized_data_maintains::{impl core::ops::function::FnOnce<(), bool> for e01::{e01::S}::__anodized_data_maintains::closure<'_0>}]
-    Source: 'examples/e01/src/lib.rs', lines 97:0-99:2 -/
+    Source: 'examples/e01/src/lib.rs', lines 98:0-100:2 -/
 @[reducible]
 def S.__anodized_data_maintains.closure.Insts.CoreOpsFunctionFnOnceTupleBool :
   core.ops.function.FnOnce S.__anodized_data_maintains.closure Unit Bool := {
@@ -1061,7 +1215,7 @@ def S.__anodized_data_maintains.closure.Insts.CoreOpsFunctionFnOnceTupleBool :
 }
 
 /-- Trait implementation: [e01::{e01::S}::__anodized_data_maintains::{impl core::ops::function::FnMut<(), bool> for e01::{e01::S}::__anodized_data_maintains::closure<'_0>}]
-    Source: 'examples/e01/src/lib.rs', lines 97:0-99:2 -/
+    Source: 'examples/e01/src/lib.rs', lines 98:0-100:2 -/
 @[reducible]
 def S.__anodized_data_maintains.closure.Insts.CoreOpsFunctionFnMutTupleBool :
   core.ops.function.FnMut S.__anodized_data_maintains.closure Unit Bool := {
@@ -1072,7 +1226,7 @@ def S.__anodized_data_maintains.closure.Insts.CoreOpsFunctionFnMutTupleBool :
 }
 
 /-- Trait implementation: [e01::{e01::S}::__anodized_data_maintains::{impl core::ops::function::Fn<(), bool> for e01::{e01::S}::__anodized_data_maintains::closure<'_0>}]
-    Source: 'examples/e01/src/lib.rs', lines 97:0-99:2 -/
+    Source: 'examples/e01/src/lib.rs', lines 98:0-100:2 -/
 @[reducible]
 def S.__anodized_data_maintains.closure.Insts.CoreOpsFunctionFnTupleBool :
   core.ops.function.Fn S.__anodized_data_maintains.closure Unit Bool := {
@@ -1083,7 +1237,7 @@ def S.__anodized_data_maintains.closure.Insts.CoreOpsFunctionFnTupleBool :
 }
 
 /-- [e01::{e01::S}::__anodized_data_maintains]:
-    Source: 'examples/e01/src/lib.rs', lines 97:0-99:2 -/
+    Source: 'examples/e01/src/lib.rs', lines 98:0-100:2 -/
 def S.__anodized_data_maintains (self : S) : Result Bool := do
   S.__anodized_data_maintains.closure.Insts.CoreOpsFunctionFnTupleBool.call
     self ()
